re-extract F*

libcrux-ml-kem/proofs/fstar/extraction/Libcrux_ml_kem.Hash_functions.Avx2.fsti
@@ -6,9 +6,7 @@ open FStar.Mul
 /// The state.
 /// It's only used for SHAKE128.
 /// All other functions don't actually use any members.
-type t_Simd256Hash = {
-  f_shake128_state:Libcrux_sha3.Generic_keccak.t_KeccakState (sz 4) Core.Core_arch.X86.t____m256i
-}
+type t_Simd256Hash = { f_shake128_state:Libcrux_sha3.Avx2.X4.Incremental.t_KeccakState4 }
 
 [@@ FStar.Tactics.Typeclasses.tcinstance]
 let impl (v_K: usize) : Libcrux_ml_kem.Hash_functions.t_Hash t_Simd256Hash v_K =
@@ -35,7 +33,7 @@ let impl (v_K: usize) : Libcrux_ml_kem.Hash_functions.t_Hash t_Simd256Hash v_K =
     =
     (fun (v_LEN: usize) (input: t_Slice u8) ->
         let digest:t_Array u8 v_LEN = Rust_primitives.Hax.repeat 0uy v_LEN in
-        let digest:t_Array u8 v_LEN = Libcrux_sha3.Portable.shake256 v_LEN digest input in
+        let digest:t_Array u8 v_LEN = Libcrux_sha3.Portable.shake256 digest input in
         digest);
     f_PRFxN_pre = (fun (v_LEN: usize) (input: t_Array (t_Array u8 (sz 33)) v_K) -> true);
     f_PRFxN_post
@@ -43,7 +41,7 @@ let impl (v_K: usize) : Libcrux_ml_kem.Hash_functions.t_Hash t_Simd256Hash v_K =
     (fun
         (v_LEN: usize)
         (input: t_Array (t_Array u8 (sz 33)) v_K)
-        (out: t_Array (t_Array u8 v_LEN) v_K)
+        (out1: t_Array (t_Array u8 v_LEN) v_K)
         ->
         true);
     f_PRFxN
@@ -62,7 +60,11 @@ let impl (v_K: usize) : Libcrux_ml_kem.Hash_functions.t_Hash t_Simd256Hash v_K =
             in
             ()
         in
-        Libcrux_sha3.Avx2.X4.shake256xN v_LEN v_K input);
+        let out:t_Array (t_Array u8 v_LEN) v_K =
+          Rust_primitives.Hax.repeat (Rust_primitives.Hax.repeat 0uy v_LEN <: t_Array u8 v_LEN) v_K
+        in
+        let _:Prims.unit = "failure" in
+        out);
     f_shake128_init_absorb_pre = (fun (input: t_Array (t_Array u8 (sz 34)) v_K) -> true);
     f_shake128_init_absorb_post
     =
@@ -83,9 +85,10 @@ let impl (v_K: usize) : Libcrux_ml_kem.Hash_functions.t_Hash t_Simd256Hash v_K =
             in
             ()
         in
-        let state:Libcrux_sha3.Generic_keccak.t_KeccakState (sz 4) Core.Core_arch.X86.t____m256i =
-          Libcrux_sha3.Avx2.X4.Incremental.shake128_absorb_finalxN v_K input
+        let state:Libcrux_sha3.Avx2.X4.Incremental.t_KeccakState4 =
+          Libcrux_sha3.Avx2.X4.Incremental.shake128_init ()
         in
+        let state:Libcrux_sha3.Avx2.X4.Incremental.t_KeccakState4 = "failure" in
         { f_shake128_state = state } <: t_Simd256Hash);
     f_shake128_squeeze_three_blocks_pre = (fun (self: t_Simd256Hash) -> true);
     f_shake128_squeeze_three_blocks_post
@@ -107,12 +110,12 @@ let impl (v_K: usize) : Libcrux_ml_kem.Hash_functions.t_Hash t_Simd256Hash v_K =
             in
             ()
         in
-        let tmp0, out:(Libcrux_sha3.Generic_keccak.t_KeccakState (sz 4)
-            Core.Core_arch.X86.t____m256i &
-          t_Array (t_Array u8 (sz 504)) v_K) =
-          Libcrux_sha3.Avx2.X4.Incremental.shake128_squeeze3xN (sz 504) v_K self.f_shake128_state
+        let out:t_Array (t_Array u8 (sz 504)) v_K =
+          Rust_primitives.Hax.repeat (Rust_primitives.Hax.repeat 0uy (sz 504) <: t_Array u8 (sz 504)
+            )
+            v_K
         in
-        let self:t_Simd256Hash = { self with f_shake128_state = tmp0 } <: t_Simd256Hash in
+        let _:Prims.unit = "failure" in
         let hax_temp_output:t_Array (t_Array u8 (sz 504)) v_K = out in
         self, hax_temp_output <: (t_Simd256Hash & t_Array (t_Array u8 (sz 504)) v_K));
     f_shake128_squeeze_block_pre = (fun (self: t_Simd256Hash) -> true);
@@ -135,11 +138,11 @@ let impl (v_K: usize) : Libcrux_ml_kem.Hash_functions.t_Hash t_Simd256Hash v_K =
           in
           ()
       in
-      let tmp0, out:(Libcrux_sha3.Generic_keccak.t_KeccakState (sz 4) Core.Core_arch.X86.t____m256i &
-        t_Array (t_Array u8 (sz 168)) v_K) =
-        Libcrux_sha3.Avx2.X4.Incremental.shake128_squeezexN (sz 168) v_K self.f_shake128_state
+      let out:t_Array (t_Array u8 (sz 168)) v_K =
+        Rust_primitives.Hax.repeat (Rust_primitives.Hax.repeat 0uy (sz 168) <: t_Array u8 (sz 168))
+          v_K
       in
-      let self:t_Simd256Hash = { self with f_shake128_state = tmp0 } <: t_Simd256Hash in
+      let _:Prims.unit = "failure" in
       let hax_temp_output:t_Array (t_Array u8 (sz 168)) v_K = out in
       self, hax_temp_output <: (t_Simd256Hash & t_Array (t_Array u8 (sz 168)) v_K)
   }
