libcrux-ml-kem/proofs/fstar/extraction/Libcrux_ml_kem.Hash_functions.Neon.fsti
@@ -7,8 +7,7 @@ open FStar.Mul
 /// It's only used for SHAKE128.
 /// All other functions don't actually use any members.
 type t_Simd128Hash = {
-  f_shake128_state:t_Array (t_Array (Libcrux_sha3.Generic_keccak.t_KeccakState (sz 1) u64) (sz 2))
-    (sz 2)
+  f_shake128_state:t_Array Libcrux_sha3.Neon.X2.Incremental.t_KeccakState2 (sz 2)
 }
 
 [@@ FStar.Tactics.Typeclasses.tcinstance]
@@ -36,7 +35,13 @@ let impl (v_K: usize) : Libcrux_ml_kem.Hash_functions.t_Hash t_Simd128Hash v_K =
     =
     (fun (v_LEN: usize) (input: t_Slice u8) ->
         let digest:t_Array u8 v_LEN = Rust_primitives.Hax.repeat 0uy v_LEN in
-        let digest:t_Array u8 v_LEN = Libcrux_sha3.Neon.shake256 v_LEN digest input in
+        let dummy:t_Array u8 v_LEN = Rust_primitives.Hax.repeat 0uy v_LEN in
+        let tmp0, tmp1:(t_Array u8 v_LEN & t_Array u8 v_LEN) =
+          Libcrux_sha3.Neon.X2.shake256 input input digest dummy
+        in
+        let digest:t_Array u8 v_LEN = tmp0 in
+        let dummy:t_Array u8 v_LEN = tmp1 in
+        let _:Prims.unit = () in
         digest);
     f_PRFxN_pre = (fun (v_LEN: usize) (input: t_Array (t_Array u8 (sz 33)) v_K) -> true);
     f_PRFxN_post
@@ -44,7 +49,7 @@ let impl (v_K: usize) : Libcrux_ml_kem.Hash_functions.t_Hash t_Simd128Hash v_K =
     (fun
         (v_LEN: usize)
         (input: t_Array (t_Array u8 (sz 33)) v_K)
-        (out: t_Array (t_Array u8 v_LEN) v_K)
+        (out1: t_Array (t_Array u8 v_LEN) v_K)
         ->
         true);
     f_PRFxN
@@ -63,7 +68,11 @@ let impl (v_K: usize) : Libcrux_ml_kem.Hash_functions.t_Hash t_Simd128Hash v_K =
             in
             ()
         in
-        Libcrux_sha3.Neon.X2.shake256xN v_LEN v_K input);
+        let out:t_Array (t_Array u8 v_LEN) v_K =
+          Rust_primitives.Hax.repeat (Rust_primitives.Hax.repeat 0uy v_LEN <: t_Array u8 v_LEN) v_K
+        in
+        let _:Prims.unit = "failure" in
+        out);
     f_shake128_init_absorb_pre = (fun (input: t_Array (t_Array u8 (sz 34)) v_K) -> true);
     f_shake128_init_absorb_post
     =
@@ -84,10 +93,17 @@ let impl (v_K: usize) : Libcrux_ml_kem.Hash_functions.t_Hash t_Simd128Hash v_K =
             in
             ()
         in
-        let state:t_Array (t_Array (Libcrux_sha3.Generic_keccak.t_KeccakState (sz 1) u64) (sz 2))
-          (sz 2) =
-          Libcrux_sha3.Neon.X2.Incremental.shake128_absorb_finalxN v_K input
+        let state:t_Array Libcrux_sha3.Neon.X2.Incremental.t_KeccakState2 (sz 2) =
+          let list =
+            [
+              Libcrux_sha3.Neon.X2.Incremental.shake128_init ();
+              Libcrux_sha3.Neon.X2.Incremental.shake128_init ()
+            ]
+          in
+          FStar.Pervasives.assert_norm (Prims.eq2 (List.Tot.length list) 2);
+          Rust_primitives.Hax.array_of_list 2 list
         in
+        let state:t_Array Libcrux_sha3.Neon.X2.Incremental.t_KeccakState2 (sz 2) = "failure" in
         { f_shake128_state = state } <: t_Simd128Hash);
     f_shake128_squeeze_three_blocks_pre = (fun (self: t_Simd128Hash) -> true);
     f_shake128_squeeze_three_blocks_post
@@ -109,18 +125,18 @@ let impl (v_K: usize) : Libcrux_ml_kem.Hash_functions.t_Hash t_Simd128Hash v_K =
             in
             ()
         in
-        let tmp0, out:(t_Array
-            (t_Array (Libcrux_sha3.Generic_keccak.t_KeccakState (sz 1) u64) (sz 2)) (sz 2) &
-          t_Array (t_Array u8 (sz 504)) v_K) =
-          Libcrux_sha3.Neon.X2.Incremental.shake128_squeeze3xN (sz 504) v_K self.f_shake128_state
+        let out:t_Array (t_Array u8 (sz 504)) v_K =
+          Rust_primitives.Hax.repeat (Rust_primitives.Hax.repeat 0uy (sz 504) <: t_Array u8 (sz 504)
+            )
+            v_K
         in
-        let self:t_Simd128Hash = { self with f_shake128_state = tmp0 } <: t_Simd128Hash in
+        let _:Prims.unit = "failure" in
         let hax_temp_output:t_Array (t_Array u8 (sz 504)) v_K = out in
         self, hax_temp_output <: (t_Simd128Hash & t_Array (t_Array u8 (sz 504)) v_K));
     f_shake128_squeeze_block_pre = (fun (self: t_Simd128Hash) -> true);
     f_shake128_squeeze_block_post
     =
-    (fun (self: t_Simd128Hash) (out1: (t_Simd128Hash & t_Array (t_Array u8 (sz 168)) v_K)) -> true);
+    (fun (self: t_Simd128Hash) (out4: (t_Simd128Hash & t_Array (t_Array u8 (sz 168)) v_K)) -> true);
     f_shake128_squeeze_block
     =
     fun (self: t_Simd128Hash) ->
@@ -137,12 +153,11 @@ let impl (v_K: usize) : Libcrux_ml_kem.Hash_functions.t_Hash t_Simd128Hash v_K =
           in
           ()
       in
-      let tmp0, out:(t_Array (t_Array (Libcrux_sha3.Generic_keccak.t_KeccakState (sz 1) u64) (sz 2))
-          (sz 2) &
-        t_Array (t_Array u8 (sz 168)) v_K) =
-        Libcrux_sha3.Neon.X2.Incremental.shake128_squeezexN (sz 168) v_K self.f_shake128_state
+      let out:t_Array (t_Array u8 (sz 168)) v_K =
+        Rust_primitives.Hax.repeat (Rust_primitives.Hax.repeat 0uy (sz 168) <: t_Array u8 (sz 168))
+          v_K
       in
-      let self:t_Simd128Hash = { self with f_shake128_state = tmp0 } <: t_Simd128Hash in
+      let out, self:(t_Array (t_Array u8 (sz 168)) v_K & t_Simd128Hash) = "failure" in
       let hax_temp_output:t_Array (t_Array u8 (sz 168)) v_K = out in
       self, hax_temp_output <: (t_Simd128Hash & t_Array (t_Array u8 (sz 168)) v_K)
   }
