libcrux-ml-kem/proofs/fstar/extraction/Libcrux_ml_kem.Mlkem512.fst
@@ -7,12 +7,20 @@ let decapsulate
       (private_key: Libcrux_ml_kem.Types.t_MlKemPrivateKey (sz 1632))
       (ciphertext: Libcrux_ml_kem.Types.t_MlKemCiphertext (sz 768))
      =
-  Libcrux_ml_kem.Ind_cca.decapsulate (sz 2) (sz 1632) (sz 768) (sz 800) (sz 768) (sz 768) (sz 640)
-    (sz 128) (sz 10) (sz 4) (sz 320) (sz 3) (sz 192) (sz 2) (sz 128) (sz 800) private_key ciphertext
+  Libcrux_ml_kem.Ind_cca.Multiplexing.decapsulate (sz 2) (sz 1632) (sz 768) (sz 800) (sz 768)
+    (sz 768) (sz 640) (sz 128) (sz 10) (sz 4) (sz 320) (sz 3) (sz 192) (sz 2) (sz 128) (sz 800)
+    private_key ciphertext
+
+let encapsulate
+      (public_key: Libcrux_ml_kem.Types.t_MlKemPublicKey (sz 800))
+      (randomness: t_Array u8 (sz 32))
+     =
+  Libcrux_ml_kem.Ind_cca.Multiplexing.encapsulate (sz 2) (sz 768) (sz 800) (sz 768) (sz 640)
+    (sz 128) (sz 10) (sz 4) (sz 320) (sz 3) (sz 192) (sz 2) (sz 128) public_key randomness
 
 let validate_public_key (public_key: Libcrux_ml_kem.Types.t_MlKemPublicKey (sz 800)) =
   if
-    Libcrux_ml_kem.Ind_cca.validate_public_key (sz 2)
+    Libcrux_ml_kem.Ind_cca.Multiplexing.validate_public_key (sz 2)
       (sz 768)
       (sz 800)
       public_key.Libcrux_ml_kem.Types.f_value
@@ -23,15 +31,8 @@ let validate_public_key (public_key: Libcrux_ml_kem.Types.t_MlKemPublicKey (sz 8
   else
     Core.Option.Option_None <: Core.Option.t_Option (Libcrux_ml_kem.Types.t_MlKemPublicKey (sz 800))
 
-let encapsulate
-      (public_key: Libcrux_ml_kem.Types.t_MlKemPublicKey (sz 800))
-      (randomness: t_Array u8 (sz 32))
-     =
-  Libcrux_ml_kem.Ind_cca.encapsulate (sz 2) (sz 768) (sz 800) (sz 768) (sz 640) (sz 128) (sz 10)
-    (sz 4) (sz 320) (sz 3) (sz 192) (sz 2) (sz 128) public_key randomness
-
 let generate_key_pair (randomness: t_Array u8 (sz 64)) =
-  Libcrux_ml_kem.Ind_cca.generate_keypair (sz 2)
+  Libcrux_ml_kem.Ind_cca.Multiplexing.generate_keypair (sz 2)
     (sz 768)
     (sz 1632)
     (sz 800)
