libcrux-ml-kem/proofs/fstar/extraction/Libcrux_ml_kem.Vector.Avx2.Arithmetic.fst
@@ -1,0 +1,150 @@
+module Libcrux_ml_kem.Vector.Avx2.Arithmetic
+#set-options "--fuel 0 --ifuel 1 --z3rlimit 15"
+open Core
+open FStar.Mul
+
+let add (lhs rhs: Core.Core_arch.X86.t____m256i) = Libcrux_intrinsics.Avx2.mm256_add_epi16 lhs rhs
+
+let bitwise_and_with_constant (vector: Core.Core_arch.X86.t____m256i) (constant: i16) =
+  Libcrux_intrinsics.Avx2.mm256_and_si256 vector
+    (Libcrux_intrinsics.Avx2.mm256_set1_epi16 constant <: Core.Core_arch.X86.t____m256i)
+
+let multiply_by_constant (vector: Core.Core_arch.X86.t____m256i) (constant: i16) =
+  Libcrux_intrinsics.Avx2.mm256_mullo_epi16 vector
+    (Libcrux_intrinsics.Avx2.mm256_set1_epi16 constant <: Core.Core_arch.X86.t____m256i)
+
+let shift_right (v_SHIFT_BY: i32) (vector: Core.Core_arch.X86.t____m256i) =
+  Libcrux_intrinsics.Avx2.mm256_srai_epi16 v_SHIFT_BY vector
+
+let sub (lhs rhs: Core.Core_arch.X86.t____m256i) = Libcrux_intrinsics.Avx2.mm256_sub_epi16 lhs rhs
+
+let barrett_reduce (vector: Core.Core_arch.X86.t____m256i) =
+  let t:Core.Core_arch.X86.t____m256i =
+    Libcrux_intrinsics.Avx2.mm256_mulhi_epi16 vector
+      (Libcrux_intrinsics.Avx2.mm256_set1_epi16 v_BARRETT_MULTIPLIER
+        <:
+        Core.Core_arch.X86.t____m256i)
+  in
+  let t:Core.Core_arch.X86.t____m256i =
+    Libcrux_intrinsics.Avx2.mm256_add_epi16 t
+      (Libcrux_intrinsics.Avx2.mm256_set1_epi16 512s <: Core.Core_arch.X86.t____m256i)
+  in
+  let quotient:Core.Core_arch.X86.t____m256i = Libcrux_intrinsics.Avx2.mm256_srai_epi16 10l t in
+  let quotient_times_field_modulus:Core.Core_arch.X86.t____m256i =
+    Libcrux_intrinsics.Avx2.mm256_mullo_epi16 quotient
+      (Libcrux_intrinsics.Avx2.mm256_set1_epi16 Libcrux_ml_kem.Vector.Traits.v_FIELD_MODULUS
+        <:
+        Core.Core_arch.X86.t____m256i)
+  in
+  Libcrux_intrinsics.Avx2.mm256_sub_epi16 vector quotient_times_field_modulus
+
+let cond_subtract_3329_ (vector: Core.Core_arch.X86.t____m256i) =
+  let field_modulus:Core.Core_arch.X86.t____m256i =
+    Libcrux_intrinsics.Avx2.mm256_set1_epi16 Libcrux_ml_kem.Vector.Traits.v_FIELD_MODULUS
+  in
+  let vv_minus_field_modulus:Core.Core_arch.X86.t____m256i =
+    Libcrux_intrinsics.Avx2.mm256_sub_epi16 vector field_modulus
+  in
+  let sign_mask:Core.Core_arch.X86.t____m256i =
+    Libcrux_intrinsics.Avx2.mm256_srai_epi16 15l vv_minus_field_modulus
+  in
+  let conditional_add_field_modulus:Core.Core_arch.X86.t____m256i =
+    Libcrux_intrinsics.Avx2.mm256_and_si256 sign_mask field_modulus
+  in
+  Libcrux_intrinsics.Avx2.mm256_add_epi16 vv_minus_field_modulus conditional_add_field_modulus
+
+let montgomery_multiply_by_constant (vector: Core.Core_arch.X86.t____m256i) (constant: i16) =
+  let constant:Core.Core_arch.X86.t____m256i = Libcrux_intrinsics.Avx2.mm256_set1_epi16 constant in
+  let value_low:Core.Core_arch.X86.t____m256i =
+    Libcrux_intrinsics.Avx2.mm256_mullo_epi16 vector constant
+  in
+  let k:Core.Core_arch.X86.t____m256i =
+    Libcrux_intrinsics.Avx2.mm256_mullo_epi16 value_low
+      (Libcrux_intrinsics.Avx2.mm256_set1_epi16 (cast (Libcrux_ml_kem.Vector.Traits.v_INVERSE_OF_MODULUS_MOD_MONTGOMERY_R
+                <:
+                u32)
+            <:
+            i16)
+        <:
+        Core.Core_arch.X86.t____m256i)
+  in
+  let k_times_modulus:Core.Core_arch.X86.t____m256i =
+    Libcrux_intrinsics.Avx2.mm256_mulhi_epi16 k
+      (Libcrux_intrinsics.Avx2.mm256_set1_epi16 Libcrux_ml_kem.Vector.Traits.v_FIELD_MODULUS
+        <:
+        Core.Core_arch.X86.t____m256i)
+  in
+  let value_high:Core.Core_arch.X86.t____m256i =
+    Libcrux_intrinsics.Avx2.mm256_mulhi_epi16 vector constant
+  in
+  Libcrux_intrinsics.Avx2.mm256_sub_epi16 value_high k_times_modulus
+
+let montgomery_multiply_by_constants (v c: Core.Core_arch.X86.t____m256i) =
+  let value_low:Core.Core_arch.X86.t____m256i = Libcrux_intrinsics.Avx2.mm256_mullo_epi16 v c in
+  let k:Core.Core_arch.X86.t____m256i =
+    Libcrux_intrinsics.Avx2.mm256_mullo_epi16 value_low
+      (Libcrux_intrinsics.Avx2.mm256_set1_epi16 (cast (Libcrux_ml_kem.Vector.Traits.v_INVERSE_OF_MODULUS_MOD_MONTGOMERY_R
+                <:
+                u32)
+            <:
+            i16)
+        <:
+        Core.Core_arch.X86.t____m256i)
+  in
+  let k_times_modulus:Core.Core_arch.X86.t____m256i =
+    Libcrux_intrinsics.Avx2.mm256_mulhi_epi16 k
+      (Libcrux_intrinsics.Avx2.mm256_set1_epi16 Libcrux_ml_kem.Vector.Traits.v_FIELD_MODULUS
+        <:
+        Core.Core_arch.X86.t____m256i)
+  in
+  let value_high:Core.Core_arch.X86.t____m256i = Libcrux_intrinsics.Avx2.mm256_mulhi_epi16 v c in
+  Libcrux_intrinsics.Avx2.mm256_sub_epi16 value_high k_times_modulus
+
+let montgomery_multiply_m128i_by_constants (v c: Core.Core_arch.X86.t____m128i) =
+  let value_low:Core.Core_arch.X86.t____m128i = Libcrux_intrinsics.Avx2.mm_mullo_epi16 v c in
+  let k:Core.Core_arch.X86.t____m128i =
+    Libcrux_intrinsics.Avx2.mm_mullo_epi16 value_low
+      (Libcrux_intrinsics.Avx2.mm_set1_epi16 (cast (Libcrux_ml_kem.Vector.Traits.v_INVERSE_OF_MODULUS_MOD_MONTGOMERY_R
+                <:
+                u32)
+            <:
+            i16)
+        <:
+        Core.Core_arch.X86.t____m128i)
+  in
+  let k_times_modulus:Core.Core_arch.X86.t____m128i =
+    Libcrux_intrinsics.Avx2.mm_mulhi_epi16 k
+      (Libcrux_intrinsics.Avx2.mm_set1_epi16 Libcrux_ml_kem.Vector.Traits.v_FIELD_MODULUS
+        <:
+        Core.Core_arch.X86.t____m128i)
+  in
+  let value_high:Core.Core_arch.X86.t____m128i = Libcrux_intrinsics.Avx2.mm_mulhi_epi16 v c in
+  Libcrux_intrinsics.Avx2.mm_sub_epi16 value_high k_times_modulus
+
+let montgomery_reduce_i32s (v: Core.Core_arch.X86.t____m256i) =
+  let k:Core.Core_arch.X86.t____m256i =
+    Libcrux_intrinsics.Avx2.mm256_mullo_epi16 v
+      (Libcrux_intrinsics.Avx2.mm256_set1_epi32 (cast (Libcrux_ml_kem.Vector.Traits.v_INVERSE_OF_MODULUS_MOD_MONTGOMERY_R
+                <:
+                u32)
+            <:
+            i32)
+        <:
+        Core.Core_arch.X86.t____m256i)
+  in
+  let k_times_modulus:Core.Core_arch.X86.t____m256i =
+    Libcrux_intrinsics.Avx2.mm256_mulhi_epi16 k
+      (Libcrux_intrinsics.Avx2.mm256_set1_epi32 (cast (Libcrux_ml_kem.Vector.Traits.v_FIELD_MODULUS
+                <:
+                i16)
+            <:
+            i32)
+        <:
+        Core.Core_arch.X86.t____m256i)
+  in
+  let value_high:Core.Core_arch.X86.t____m256i = Libcrux_intrinsics.Avx2.mm256_srli_epi32 16l v in
+  let result:Core.Core_arch.X86.t____m256i =
+    Libcrux_intrinsics.Avx2.mm256_sub_epi16 value_high k_times_modulus
+  in
+  let result:Core.Core_arch.X86.t____m256i = Libcrux_intrinsics.Avx2.mm256_slli_epi32 16l result in
+  Libcrux_intrinsics.Avx2.mm256_srai_epi32 16l result
