libcrux-ml-kem/proofs/fstar/extraction/Libcrux_ml_kem.Vector.fsti
@@ -1,0 +1,729 @@
+module Libcrux_ml_kem.Vector
+#set-options "--fuel 0 --ifuel 1 --z3rlimit 15"
+open Core
+open FStar.Mul
+
+let _ =
+  (* This module has implicit dependencies, here we make them explicit. *)
+  (* The implicit dependencies arise from typeclasses instances. *)
+  let open Libcrux_ml_kem.Vector.Portable in
+  ()
+
+/// Values having this type hold a representative 'x' of the Kyber field.
+/// We use 'fe' as a shorthand for this type.
+unfold
+let t_FieldElement = i16
+
+/// If 'x' denotes a value of type `fe`, values having this type hold a
+/// representative y ≡ x·MONTGOMERY_R (mod FIELD_MODULUS).
+/// We use 'fer' as a shorthand for this type.
+unfold
+let t_FieldElementTimesMontgomeryR = i16
+
+/// If 'x' denotes a value of type `fe`, values having this type hold a
+/// representative y ≡ x·MONTGOMERY_R^(-1) (mod FIELD_MODULUS).
+/// We use 'mfe' as a shorthand for this type
+unfold
+let t_MontgomeryFieldElement = i16
+
+/// This is calculated as ⌊(BARRETT_R / FIELD_MODULUS) + 1/2⌋
+let v_BARRETT_MULTIPLIER: i32 = Rust_primitives.Hax.dropped_body
+
+let v_BARRETT_R: i32 = Rust_primitives.Hax.dropped_body
+
+let v_BARRETT_SHIFT: i32 = Rust_primitives.Hax.dropped_body
+
+let v_MONTGOMERY_R: i32 = Rust_primitives.Hax.dropped_body
+
+let v_MONTGOMERY_SHIFT: u8 = Rust_primitives.Hax.dropped_body
+
+/// Signed Barrett Reduction
+/// Given an input `value`, `barrett_reduce` outputs a representative `result`
+/// such that:
+/// - result ≡ value (mod FIELD_MODULUS)
+/// - the absolute value of `result` is bound as follows:
+/// `|result| ≤ FIELD_MODULUS / 2 · (|value|/BARRETT_R + 1)
+/// In particular, if `|value| < BARRETT_R`, then `|result| < FIELD_MODULUS`.
+val barrett_reduce_element (value: i16)
+    : Prims.Pure i16
+      (requires
+        (Core.Convert.f_from #i32 #i16 value <: i32) >. (Core.Ops.Arith.Neg.neg v_BARRETT_R <: i32) &&
+        (Core.Convert.f_from #i32 #i16 value <: i32) <. v_BARRETT_R)
+      (ensures
+        fun result ->
+          let result:i16 = result in
+          result >. (Core.Ops.Arith.Neg.neg Libcrux_ml_kem.Vector.Traits.v_FIELD_MODULUS <: i16) &&
+          result <. Libcrux_ml_kem.Vector.Traits.v_FIELD_MODULUS)
+
+val compress_ciphertext_coefficient (coefficient_bits: u8) (fe: u16)
+    : Prims.Pure i16
+      (requires
+        Rust_primitives.Hax.failure "(AST import) Fatal error: something we considered as impossible occurred! Please report this by submitting an issue on GitHub!\nDetails: [import_thir:literal] got an error literal: this means the Rust compiler or Hax's frontend probably reported errors above.\n"
+          "{ Types.attributes = [];\n  contents =\n  Types.Literal {\n    lit =\n    { Types.node = Types.Err;\n      span =\n      { Types.filename =\n        (Types.Real (Types.LocalPath \"libcrux-ml-kem/src/lib.rs\"));\n        hi = { Types.col = \"0\"; line = \"1\" };\n        lo = { Types.col = \"0\"; line = \"1\" } }\n      };\n    neg = false};\n  hir_id = None;\n  span =\n  { Types.filename =\n    (Types.Real (Types.LocalPath \"libcrux-ml-kem/src/vector.rs\"));\n    hi = { Types.col = \"55\"; line = \"182\" };\n    lo = { Types.col = \"4\"; line = \"177\" } };\n  ty = Types.Never }"
+        )
+      (ensures
+        fun result ->
+          let result:i16 = result in
+          result >=. 0s &&
+          result <. (Core.Num.impl__i16__pow 2s (cast (coefficient_bits <: u8) <: u32) <: i16))
+
+/// The `compress_*` functions implement the `Compress` function specified in the NIST FIPS
+/// 203 standard (Page 18, Expression 4.5), which is defined as:
+/// ```plaintext
+/// Compress_d: ℤq -> ℤ_{2ᵈ}
+/// Compress_d(x) = ⌈(2ᵈ/q)·x⌋
+/// ```
+/// Since `⌈x⌋ = ⌊x + 1/2⌋` we have:
+/// ```plaintext
+/// Compress_d(x) = ⌊(2ᵈ/q)·x + 1/2⌋
+///               = ⌊(2^{d+1}·x + q) / 2q⌋
+/// ```
+/// For further information about the function implementations, consult the
+/// `implementation_notes.pdf` document in this directory.
+/// The NIST FIPS 203 standard can be found at
+/// <https://csrc.nist.gov/pubs/fips/203/ipd>.
+val compress_message_coefficient (fe: u16)
+    : Prims.Pure u8
+      (requires
+        Rust_primitives.Hax.failure "(AST import) Fatal error: something we considered as impossible occurred! Please report this by submitting an issue on GitHub!\nDetails: [import_thir:literal] got an error literal: this means the Rust compiler or Hax's frontend probably reported errors above.\n"
+          "{ Types.attributes = [];\n  contents =\n  Types.Literal {\n    lit =\n    { Types.node = Types.Err;\n      span =\n      { Types.filename =\n        (Types.Real (Types.LocalPath \"libcrux-ml-kem/src/lib.rs\"));\n        hi = { Types.col = \"0\"; line = \"1\" };\n        lo = { Types.col = \"0\"; line = \"1\" } }\n      };\n    neg = false};\n  hir_id = None;\n  span =\n  { Types.filename =\n    (Types.Real (Types.LocalPath \"libcrux-ml-kem/src/vector.rs\"));\n    hi = { Types.col = \"80\"; line = \"146\" };\n    lo = { Types.col = \"16\"; line = \"146\" } };\n  ty = Types.Never }"
+        )
+      (ensures
+        fun result ->
+          let result:u8 = result in
+          Hax_lib.implies ((833us <=. fe <: bool) && (fe <=. 2596us <: bool))
+            (fun temp_0_ ->
+                let _:Prims.unit = temp_0_ in
+                result =. 1uy <: bool) &&
+          Hax_lib.implies (~.((833us <=. fe <: bool) && (fe <=. 2596us <: bool)) <: bool)
+            (fun temp_0_ ->
+                let _:Prims.unit = temp_0_ in
+                result =. 0uy <: bool))
+
+val get_n_least_significant_bits (n: u8) (value: u32)
+    : Prims.Pure u32
+      (requires n =. 4uy || n =. 5uy || n =. 10uy || n =. 11uy || n =. v_MONTGOMERY_SHIFT)
+      (ensures
+        fun result ->
+          let result:u32 = result in
+          result <. (Core.Num.impl__u32__pow 2ul (Core.Convert.f_into #u8 #u32 n <: u32) <: u32))
+
+/// If `fe` is some field element 'x' of the Kyber field and `fer` is congruent to
+/// `y · MONTGOMERY_R`, this procedure outputs a value that is congruent to
+/// `x · y`, as follows:
+///    `fe · fer ≡ x · y · MONTGOMERY_R (mod FIELD_MODULUS)`
+/// `montgomery_reduce` takes the value `x · y · MONTGOMERY_R` and outputs a representative
+/// `x · y · MONTGOMERY_R * MONTGOMERY_R^{-1} ≡ x · y (mod FIELD_MODULUS)`.
+val montgomery_multiply_fe_by_fer (fe fer: i16)
+    : Prims.Pure i16 Prims.l_True (fun _ -> Prims.l_True)
+
+/// Signed Montgomery Reduction
+/// Given an input `value`, `montgomery_reduce` outputs a representative `o`
+/// such that:
+/// - o ≡ value · MONTGOMERY_R^(-1) (mod FIELD_MODULUS)
+/// - the absolute value of `o` is bound as follows:
+/// `|result| ≤ (|value| / MONTGOMERY_R) + (FIELD_MODULUS / 2)
+/// In particular, if `|value| ≤ FIELD_MODULUS * MONTGOMERY_R`, then `|o| < (3 · FIELD_MODULUS) / 2`.
+val montgomery_reduce_element (value: i32)
+    : Prims.Pure i16
+      (requires
+        Rust_primitives.Hax.failure "(AST import) Fatal error: something we considered as impossible occurred! Please report this by submitting an issue on GitHub!\nDetails: [import_thir:literal] got an error literal: this means the Rust compiler or Hax's frontend probably reported errors above.\n"
+          "{ Types.attributes = [];\n  contents =\n  Types.Literal {\n    lit =\n    { Types.node = Types.Err;\n      span =\n      { Types.filename =\n        (Types.Real (Types.LocalPath \"libcrux-ml-kem/src/lib.rs\"));\n        hi = { Types.col = \"0\"; line = \"1\" };\n        lo = { Types.col = \"0\"; line = \"1\" } }\n      };\n    neg = false};\n  hir_id = None;\n  span =\n  { Types.filename =\n    (Types.Real (Types.LocalPath \"libcrux-ml-kem/src/vector.rs\"));\n    hi = { Types.col = \"114\"; line = \"80\" };\n    lo = { Types.col = \"16\"; line = \"80\" } };\n  ty = Types.Never }"
+        )
+      (ensures
+        fun result ->
+          let result:i16 = result in
+          result >=.
+          ((Core.Ops.Arith.Neg.neg (3s *! Libcrux_ml_kem.Vector.Traits.v_FIELD_MODULUS <: i16)
+              <:
+              i16) /!
+            2s
+            <:
+            i16) &&
+          result <=. ((3s *! Libcrux_ml_kem.Vector.Traits.v_FIELD_MODULUS <: i16) /! 2s <: i16))
+
+/// Compute the product of two Kyber binomials with respect to the
+/// modulus `X² - zeta`.
+/// This function almost implements <strong>Algorithm 11</strong> of the
+/// NIST FIPS 203 standard, which is reproduced below:
+/// ```plaintext
+/// Input:  a₀, a₁, b₀, b₁ ∈ ℤq.
+/// Input: γ ∈ ℤq.
+/// Output: c₀, c₁ ∈ ℤq.
+/// c₀ ← a₀·b₀ + a₁·b₁·γ
+/// c₁ ← a₀·b₁ + a₁·b₀
+/// return c₀, c₁
+/// ```
+/// We say "almost" because the coefficients output by this function are in
+/// the Montgomery domain (unlike in the specification).
+/// The NIST FIPS 203 standard can be found at
+/// <https://csrc.nist.gov/pubs/fips/203/ipd>.
+val ntt_multiply_binomials: (i16 & i16) -> (i16 & i16) -> zeta: i16
+  -> Prims.Pure (i16 & i16) Prims.l_True (fun _ -> Prims.l_True)
+
+val rej_sample (a: t_Slice u8) (result: t_Slice i16)
+    : Prims.Pure (t_Slice i16 & usize) Prims.l_True (fun _ -> Prims.l_True)
+
+val add (lhs rhs: Libcrux_ml_kem.Vector.Portable.t_PortableVector)
+    : Prims.Pure Libcrux_ml_kem.Vector.Portable.t_PortableVector
+      Prims.l_True
+      (fun _ -> Prims.l_True)
+
+val barrett_reduce (v: Libcrux_ml_kem.Vector.Portable.t_PortableVector)
+    : Prims.Pure Libcrux_ml_kem.Vector.Portable.t_PortableVector
+      Prims.l_True
+      (fun _ -> Prims.l_True)
+
+val bitwise_and_with_constant (v: Libcrux_ml_kem.Vector.Portable.t_PortableVector) (c: i16)
+    : Prims.Pure Libcrux_ml_kem.Vector.Portable.t_PortableVector
+      Prims.l_True
+      (fun _ -> Prims.l_True)
+
+val compress (v_COEFFICIENT_BITS: i32) (v: Libcrux_ml_kem.Vector.Portable.t_PortableVector)
+    : Prims.Pure Libcrux_ml_kem.Vector.Portable.t_PortableVector
+      Prims.l_True
+      (fun _ -> Prims.l_True)
+
+val compress_1_ (v: Libcrux_ml_kem.Vector.Portable.t_PortableVector)
+    : Prims.Pure Libcrux_ml_kem.Vector.Portable.t_PortableVector
+      Prims.l_True
+      (fun _ -> Prims.l_True)
+
+val cond_subtract_3329_ (v: Libcrux_ml_kem.Vector.Portable.t_PortableVector)
+    : Prims.Pure Libcrux_ml_kem.Vector.Portable.t_PortableVector
+      Prims.l_True
+      (fun _ -> Prims.l_True)
+
+val decompress_ciphertext_coefficient
+      (v_COEFFICIENT_BITS: i32)
+      (v: Libcrux_ml_kem.Vector.Portable.t_PortableVector)
+    : Prims.Pure Libcrux_ml_kem.Vector.Portable.t_PortableVector
+      Prims.l_True
+      (fun _ -> Prims.l_True)
+
+val deserialize_1_ (v: t_Slice u8)
+    : Prims.Pure Libcrux_ml_kem.Vector.Portable.t_PortableVector
+      Prims.l_True
+      (fun _ -> Prims.l_True)
+
+val deserialize_10_ (bytes: t_Slice u8)
+    : Prims.Pure Libcrux_ml_kem.Vector.Portable.t_PortableVector
+      Prims.l_True
+      (fun _ -> Prims.l_True)
+
+val deserialize_11_ (bytes: t_Slice u8)
+    : Prims.Pure Libcrux_ml_kem.Vector.Portable.t_PortableVector
+      Prims.l_True
+      (fun _ -> Prims.l_True)
+
+val deserialize_12_ (bytes: t_Slice u8)
+    : Prims.Pure Libcrux_ml_kem.Vector.Portable.t_PortableVector
+      Prims.l_True
+      (fun _ -> Prims.l_True)
+
+val deserialize_4_ (bytes: t_Slice u8)
+    : Prims.Pure Libcrux_ml_kem.Vector.Portable.t_PortableVector
+      Prims.l_True
+      (fun _ -> Prims.l_True)
+
+val deserialize_5_ (bytes: t_Slice u8)
+    : Prims.Pure Libcrux_ml_kem.Vector.Portable.t_PortableVector
+      Prims.l_True
+      (fun _ -> Prims.l_True)
+
+val from_i16_array (array: t_Slice i16)
+    : Prims.Pure Libcrux_ml_kem.Vector.Portable.t_PortableVector
+      Prims.l_True
+      (fun _ -> Prims.l_True)
+
+val inv_ntt_layer_1_step
+      (v: Libcrux_ml_kem.Vector.Portable.t_PortableVector)
+      (zeta0 zeta1 zeta2 zeta3: i16)
+    : Prims.Pure Libcrux_ml_kem.Vector.Portable.t_PortableVector
+      Prims.l_True
+      (fun _ -> Prims.l_True)
+
+val inv_ntt_layer_2_step (v: Libcrux_ml_kem.Vector.Portable.t_PortableVector) (zeta0 zeta1: i16)
+    : Prims.Pure Libcrux_ml_kem.Vector.Portable.t_PortableVector
+      Prims.l_True
+      (fun _ -> Prims.l_True)
+
+val inv_ntt_layer_3_step (v: Libcrux_ml_kem.Vector.Portable.t_PortableVector) (zeta: i16)
+    : Prims.Pure Libcrux_ml_kem.Vector.Portable.t_PortableVector
+      Prims.l_True
+      (fun _ -> Prims.l_True)
+
+val montgomery_multiply_by_constant (v: Libcrux_ml_kem.Vector.Portable.t_PortableVector) (c: i16)
+    : Prims.Pure Libcrux_ml_kem.Vector.Portable.t_PortableVector
+      Prims.l_True
+      (fun _ -> Prims.l_True)
+
+val multiply_by_constant (v: Libcrux_ml_kem.Vector.Portable.t_PortableVector) (c: i16)
+    : Prims.Pure Libcrux_ml_kem.Vector.Portable.t_PortableVector
+      Prims.l_True
+      (fun _ -> Prims.l_True)
+
+val ntt_layer_1_step
+      (v: Libcrux_ml_kem.Vector.Portable.t_PortableVector)
+      (zeta0 zeta1 zeta2 zeta3: i16)
+    : Prims.Pure Libcrux_ml_kem.Vector.Portable.t_PortableVector
+      Prims.l_True
+      (fun _ -> Prims.l_True)
+
+val ntt_layer_2_step (v: Libcrux_ml_kem.Vector.Portable.t_PortableVector) (zeta0 zeta1: i16)
+    : Prims.Pure Libcrux_ml_kem.Vector.Portable.t_PortableVector
+      Prims.l_True
+      (fun _ -> Prims.l_True)
+
+val ntt_layer_3_step (v: Libcrux_ml_kem.Vector.Portable.t_PortableVector) (zeta: i16)
+    : Prims.Pure Libcrux_ml_kem.Vector.Portable.t_PortableVector
+      Prims.l_True
+      (fun _ -> Prims.l_True)
+
+val ntt_multiply
+      (lhs rhs: Libcrux_ml_kem.Vector.Portable.t_PortableVector)
+      (zeta0 zeta1 zeta2 zeta3: i16)
+    : Prims.Pure Libcrux_ml_kem.Vector.Portable.t_PortableVector
+      Prims.l_True
+      (fun _ -> Prims.l_True)
+
+val serialize_1_ (v: Libcrux_ml_kem.Vector.Portable.t_PortableVector)
+    : Prims.Pure (t_Array u8 (sz 2)) Prims.l_True (fun _ -> Prims.l_True)
+
+val serialize_10_ (v: Libcrux_ml_kem.Vector.Portable.t_PortableVector)
+    : Prims.Pure (t_Array u8 (sz 20)) Prims.l_True (fun _ -> Prims.l_True)
+
+val serialize_11_ (v: Libcrux_ml_kem.Vector.Portable.t_PortableVector)
+    : Prims.Pure (t_Array u8 (sz 22)) Prims.l_True (fun _ -> Prims.l_True)
+
+val serialize_12_ (v: Libcrux_ml_kem.Vector.Portable.t_PortableVector)
+    : Prims.Pure (t_Array u8 (sz 24)) Prims.l_True (fun _ -> Prims.l_True)
+
+val serialize_4_ (v: Libcrux_ml_kem.Vector.Portable.t_PortableVector)
+    : Prims.Pure (t_Array u8 (sz 8)) Prims.l_True (fun _ -> Prims.l_True)
+
+val serialize_5_ (v: Libcrux_ml_kem.Vector.Portable.t_PortableVector)
+    : Prims.Pure (t_Array u8 (sz 10)) Prims.l_True (fun _ -> Prims.l_True)
+
+val shift_right (v_SHIFT_BY: i32) (v: Libcrux_ml_kem.Vector.Portable.t_PortableVector)
+    : Prims.Pure Libcrux_ml_kem.Vector.Portable.t_PortableVector
+      Prims.l_True
+      (fun _ -> Prims.l_True)
+
+val sub (lhs rhs: Libcrux_ml_kem.Vector.Portable.t_PortableVector)
+    : Prims.Pure Libcrux_ml_kem.Vector.Portable.t_PortableVector
+      Prims.l_True
+      (fun _ -> Prims.l_True)
+
+val zero: Prims.unit
+  -> Prims.Pure Libcrux_ml_kem.Vector.Portable.t_PortableVector Prims.l_True (fun _ -> Prims.l_True)
+
+[@@ FStar.Tactics.Typeclasses.tcinstance]
+let impl: Libcrux_ml_kem.Vector.Traits.t_Operations Libcrux_ml_kem.Vector.Portable.t_PortableVector =
+  {
+    _super_11581440318597584651 = FStar.Tactics.Typeclasses.solve;
+    _super_9442900250278684536 = FStar.Tactics.Typeclasses.solve;
+    f_ZERO_pre = (fun (_: Prims.unit) -> true);
+    f_ZERO_post
+    =
+    (fun (_: Prims.unit) (out: Libcrux_ml_kem.Vector.Portable.t_PortableVector) -> true);
+    f_ZERO = (fun (_: Prims.unit) -> zero ());
+    f_from_i16_array_pre = (fun (array: t_Slice i16) -> true);
+    f_from_i16_array_post
+    =
+    (fun (array: t_Slice i16) (out: Libcrux_ml_kem.Vector.Portable.t_PortableVector) -> true);
+    f_from_i16_array = (fun (array: t_Slice i16) -> from_i16_array array);
+    f_add_pre
+    =
+    (fun
+        (lhs: Libcrux_ml_kem.Vector.Portable.t_PortableVector)
+        (rhs: Libcrux_ml_kem.Vector.Portable.t_PortableVector)
+        ->
+        true);
+    f_add_post
+    =
+    (fun
+        (lhs: Libcrux_ml_kem.Vector.Portable.t_PortableVector)
+        (rhs: Libcrux_ml_kem.Vector.Portable.t_PortableVector)
+        (out: Libcrux_ml_kem.Vector.Portable.t_PortableVector)
+        ->
+        true);
+    f_add
+    =
+    (fun
+        (lhs: Libcrux_ml_kem.Vector.Portable.t_PortableVector)
+        (rhs: Libcrux_ml_kem.Vector.Portable.t_PortableVector)
+        ->
+        add lhs rhs);
+    f_sub_pre
+    =
+    (fun
+        (lhs: Libcrux_ml_kem.Vector.Portable.t_PortableVector)
+        (rhs: Libcrux_ml_kem.Vector.Portable.t_PortableVector)
+        ->
+        true);
+    f_sub_post
+    =
+    (fun
+        (lhs: Libcrux_ml_kem.Vector.Portable.t_PortableVector)
+        (rhs: Libcrux_ml_kem.Vector.Portable.t_PortableVector)
+        (out: Libcrux_ml_kem.Vector.Portable.t_PortableVector)
+        ->
+        true);
+    f_sub
+    =
+    (fun
+        (lhs: Libcrux_ml_kem.Vector.Portable.t_PortableVector)
+        (rhs: Libcrux_ml_kem.Vector.Portable.t_PortableVector)
+        ->
+        sub lhs rhs);
+    f_multiply_by_constant_pre
+    =
+    (fun (v: Libcrux_ml_kem.Vector.Portable.t_PortableVector) (c: i16) -> true);
+    f_multiply_by_constant_post
+    =
+    (fun
+        (v: Libcrux_ml_kem.Vector.Portable.t_PortableVector)
+        (c: i16)
+        (out: Libcrux_ml_kem.Vector.Portable.t_PortableVector)
+        ->
+        true);
+    f_multiply_by_constant
+    =
+    (fun (v: Libcrux_ml_kem.Vector.Portable.t_PortableVector) (c: i16) -> multiply_by_constant v c);
+    f_bitwise_and_with_constant_pre
+    =
+    (fun (v: Libcrux_ml_kem.Vector.Portable.t_PortableVector) (c: i16) -> true);
+    f_bitwise_and_with_constant_post
+    =
+    (fun
+        (v: Libcrux_ml_kem.Vector.Portable.t_PortableVector)
+        (c: i16)
+        (out: Libcrux_ml_kem.Vector.Portable.t_PortableVector)
+        ->
+        true);
+    f_bitwise_and_with_constant
+    =
+    (fun (v: Libcrux_ml_kem.Vector.Portable.t_PortableVector) (c: i16) ->
+        bitwise_and_with_constant v c);
+    f_shift_right_pre
+    =
+    (fun (v_SHIFT_BY: i32) (v: Libcrux_ml_kem.Vector.Portable.t_PortableVector) -> true);
+    f_shift_right_post
+    =
+    (fun
+        (v_SHIFT_BY: i32)
+        (v: Libcrux_ml_kem.Vector.Portable.t_PortableVector)
+        (out: Libcrux_ml_kem.Vector.Portable.t_PortableVector)
+        ->
+        true);
+    f_shift_right
+    =
+    (fun (v_SHIFT_BY: i32) (v: Libcrux_ml_kem.Vector.Portable.t_PortableVector) ->
+        shift_right v_SHIFT_BY v);
+    f_cond_subtract_3329_pre = (fun (v: Libcrux_ml_kem.Vector.Portable.t_PortableVector) -> true);
+    f_cond_subtract_3329_post
+    =
+    (fun
+        (v: Libcrux_ml_kem.Vector.Portable.t_PortableVector)
+        (out: Libcrux_ml_kem.Vector.Portable.t_PortableVector)
+        ->
+        true);
+    f_cond_subtract_3329_
+    =
+    (fun (v: Libcrux_ml_kem.Vector.Portable.t_PortableVector) -> cond_subtract_3329_ v);
+    f_barrett_reduce_pre = (fun (v: Libcrux_ml_kem.Vector.Portable.t_PortableVector) -> true);
+    f_barrett_reduce_post
+    =
+    (fun
+        (v: Libcrux_ml_kem.Vector.Portable.t_PortableVector)
+        (out: Libcrux_ml_kem.Vector.Portable.t_PortableVector)
+        ->
+        true);
+    f_barrett_reduce
+    =
+    (fun (v: Libcrux_ml_kem.Vector.Portable.t_PortableVector) -> barrett_reduce v);
+    f_montgomery_multiply_by_constant_pre
+    =
+    (fun (v: Libcrux_ml_kem.Vector.Portable.t_PortableVector) (r: i16) -> true);
+    f_montgomery_multiply_by_constant_post
+    =
+    (fun
+        (v: Libcrux_ml_kem.Vector.Portable.t_PortableVector)
+        (r: i16)
+        (out: Libcrux_ml_kem.Vector.Portable.t_PortableVector)
+        ->
+        true);
+    f_montgomery_multiply_by_constant
+    =
+    (fun (v: Libcrux_ml_kem.Vector.Portable.t_PortableVector) (r: i16) ->
+        montgomery_multiply_by_constant v r);
+    f_compress_1_pre = (fun (v: Libcrux_ml_kem.Vector.Portable.t_PortableVector) -> true);
+    f_compress_1_post
+    =
+    (fun
+        (v: Libcrux_ml_kem.Vector.Portable.t_PortableVector)
+        (out: Libcrux_ml_kem.Vector.Portable.t_PortableVector)
+        ->
+        true);
+    f_compress_1_ = (fun (v: Libcrux_ml_kem.Vector.Portable.t_PortableVector) -> compress_1_ v);
+    f_compress_pre
+    =
+    (fun (v_COEFFICIENT_BITS: i32) (v: Libcrux_ml_kem.Vector.Portable.t_PortableVector) -> true);
+    f_compress_post
+    =
+    (fun
+        (v_COEFFICIENT_BITS: i32)
+        (v: Libcrux_ml_kem.Vector.Portable.t_PortableVector)
+        (out: Libcrux_ml_kem.Vector.Portable.t_PortableVector)
+        ->
+        true);
+    f_compress
+    =
+    (fun (v_COEFFICIENT_BITS: i32) (v: Libcrux_ml_kem.Vector.Portable.t_PortableVector) ->
+        compress v_COEFFICIENT_BITS v);
+    f_decompress_ciphertext_coefficient_pre
+    =
+    (fun (v_COEFFICIENT_BITS: i32) (v: Libcrux_ml_kem.Vector.Portable.t_PortableVector) -> true);
+    f_decompress_ciphertext_coefficient_post
+    =
+    (fun
+        (v_COEFFICIENT_BITS: i32)
+        (v: Libcrux_ml_kem.Vector.Portable.t_PortableVector)
+        (out: Libcrux_ml_kem.Vector.Portable.t_PortableVector)
+        ->
+        true);
+    f_decompress_ciphertext_coefficient
+    =
+    (fun (v_COEFFICIENT_BITS: i32) (v: Libcrux_ml_kem.Vector.Portable.t_PortableVector) ->
+        decompress_ciphertext_coefficient v_COEFFICIENT_BITS v);
+    f_ntt_layer_1_step_pre
+    =
+    (fun
+        (a: Libcrux_ml_kem.Vector.Portable.t_PortableVector)
+        (zeta0: i16)
+        (zeta1: i16)
+        (zeta2: i16)
+        (zeta3: i16)
+        ->
+        true);
+    f_ntt_layer_1_step_post
+    =
+    (fun
+        (a: Libcrux_ml_kem.Vector.Portable.t_PortableVector)
+        (zeta0: i16)
+        (zeta1: i16)
+        (zeta2: i16)
+        (zeta3: i16)
+        (out: Libcrux_ml_kem.Vector.Portable.t_PortableVector)
+        ->
+        true);
+    f_ntt_layer_1_step
+    =
+    (fun
+        (a: Libcrux_ml_kem.Vector.Portable.t_PortableVector)
+        (zeta0: i16)
+        (zeta1: i16)
+        (zeta2: i16)
+        (zeta3: i16)
+        ->
+        ntt_layer_1_step a zeta0 zeta1 zeta2 zeta3);
+    f_ntt_layer_2_step_pre
+    =
+    (fun (a: Libcrux_ml_kem.Vector.Portable.t_PortableVector) (zeta0: i16) (zeta1: i16) -> true);
+    f_ntt_layer_2_step_post
+    =
+    (fun
+        (a: Libcrux_ml_kem.Vector.Portable.t_PortableVector)
+        (zeta0: i16)
+        (zeta1: i16)
+        (out: Libcrux_ml_kem.Vector.Portable.t_PortableVector)
+        ->
+        true);
+    f_ntt_layer_2_step
+    =
+    (fun (a: Libcrux_ml_kem.Vector.Portable.t_PortableVector) (zeta0: i16) (zeta1: i16) ->
+        ntt_layer_2_step a zeta0 zeta1);
+    f_ntt_layer_3_step_pre
+    =
+    (fun (a: Libcrux_ml_kem.Vector.Portable.t_PortableVector) (zeta: i16) -> true);
+    f_ntt_layer_3_step_post
+    =
+    (fun
+        (a: Libcrux_ml_kem.Vector.Portable.t_PortableVector)
+        (zeta: i16)
+        (out: Libcrux_ml_kem.Vector.Portable.t_PortableVector)
+        ->
+        true);
+    f_ntt_layer_3_step
+    =
+    (fun (a: Libcrux_ml_kem.Vector.Portable.t_PortableVector) (zeta: i16) -> ntt_layer_3_step a zeta
+    );
+    f_inv_ntt_layer_1_step_pre
+    =
+    (fun
+        (a: Libcrux_ml_kem.Vector.Portable.t_PortableVector)
+        (zeta0: i16)
+        (zeta1: i16)
+        (zeta2: i16)
+        (zeta3: i16)
+        ->
+        true);
+    f_inv_ntt_layer_1_step_post
+    =
+    (fun
+        (a: Libcrux_ml_kem.Vector.Portable.t_PortableVector)
+        (zeta0: i16)
+        (zeta1: i16)
+        (zeta2: i16)
+        (zeta3: i16)
+        (out: Libcrux_ml_kem.Vector.Portable.t_PortableVector)
+        ->
+        true);
+    f_inv_ntt_layer_1_step
+    =
+    (fun
+        (a: Libcrux_ml_kem.Vector.Portable.t_PortableVector)
+        (zeta0: i16)
+        (zeta1: i16)
+        (zeta2: i16)
+        (zeta3: i16)
+        ->
+        inv_ntt_layer_1_step a zeta0 zeta1 zeta2 zeta3);
+    f_inv_ntt_layer_2_step_pre
+    =
+    (fun (a: Libcrux_ml_kem.Vector.Portable.t_PortableVector) (zeta0: i16) (zeta1: i16) -> true);
+    f_inv_ntt_layer_2_step_post
+    =
+    (fun
+        (a: Libcrux_ml_kem.Vector.Portable.t_PortableVector)
+        (zeta0: i16)
+        (zeta1: i16)
+        (out: Libcrux_ml_kem.Vector.Portable.t_PortableVector)
+        ->
+        true);
+    f_inv_ntt_layer_2_step
+    =
+    (fun (a: Libcrux_ml_kem.Vector.Portable.t_PortableVector) (zeta0: i16) (zeta1: i16) ->
+        inv_ntt_layer_2_step a zeta0 zeta1);
+    f_inv_ntt_layer_3_step_pre
+    =
+    (fun (a: Libcrux_ml_kem.Vector.Portable.t_PortableVector) (zeta: i16) -> true);
+    f_inv_ntt_layer_3_step_post
+    =
+    (fun
+        (a: Libcrux_ml_kem.Vector.Portable.t_PortableVector)
+        (zeta: i16)
+        (out: Libcrux_ml_kem.Vector.Portable.t_PortableVector)
+        ->
+        true);
+    f_inv_ntt_layer_3_step
+    =
+    (fun (a: Libcrux_ml_kem.Vector.Portable.t_PortableVector) (zeta: i16) ->
+        inv_ntt_layer_3_step a zeta);
+    f_ntt_multiply_pre
+    =
+    (fun
+        (lhs: Libcrux_ml_kem.Vector.Portable.t_PortableVector)
+        (rhs: Libcrux_ml_kem.Vector.Portable.t_PortableVector)
+        (zeta0: i16)
+        (zeta1: i16)
+        (zeta2: i16)
+        (zeta3: i16)
+        ->
+        true);
+    f_ntt_multiply_post
+    =
+    (fun
+        (lhs: Libcrux_ml_kem.Vector.Portable.t_PortableVector)
+        (rhs: Libcrux_ml_kem.Vector.Portable.t_PortableVector)
+        (zeta0: i16)
+        (zeta1: i16)
+        (zeta2: i16)
+        (zeta3: i16)
+        (out: Libcrux_ml_kem.Vector.Portable.t_PortableVector)
+        ->
+        true);
+    f_ntt_multiply
+    =
+    (fun
+        (lhs: Libcrux_ml_kem.Vector.Portable.t_PortableVector)
+        (rhs: Libcrux_ml_kem.Vector.Portable.t_PortableVector)
+        (zeta0: i16)
+        (zeta1: i16)
+        (zeta2: i16)
+        (zeta3: i16)
+        ->
+        ntt_multiply lhs rhs zeta0 zeta1 zeta2 zeta3);
+    f_serialize_1_pre = (fun (a: Libcrux_ml_kem.Vector.Portable.t_PortableVector) -> true);
+    f_serialize_1_post
+    =
+    (fun (a: Libcrux_ml_kem.Vector.Portable.t_PortableVector) (out: t_Array u8 (sz 2)) -> true);
+    f_serialize_1_ = (fun (a: Libcrux_ml_kem.Vector.Portable.t_PortableVector) -> serialize_1_ a);
+    f_deserialize_1_pre = (fun (a: t_Slice u8) -> true);
+    f_deserialize_1_post
+    =
+    (fun (a: t_Slice u8) (out: Libcrux_ml_kem.Vector.Portable.t_PortableVector) -> true);
+    f_deserialize_1_ = (fun (a: t_Slice u8) -> deserialize_1_ a);
+    f_serialize_4_pre = (fun (a: Libcrux_ml_kem.Vector.Portable.t_PortableVector) -> true);
+    f_serialize_4_post
+    =
+    (fun (a: Libcrux_ml_kem.Vector.Portable.t_PortableVector) (out: t_Array u8 (sz 8)) -> true);
+    f_serialize_4_ = (fun (a: Libcrux_ml_kem.Vector.Portable.t_PortableVector) -> serialize_4_ a);
+    f_deserialize_4_pre = (fun (a: t_Slice u8) -> true);
+    f_deserialize_4_post
+    =
+    (fun (a: t_Slice u8) (out: Libcrux_ml_kem.Vector.Portable.t_PortableVector) -> true);
+    f_deserialize_4_ = (fun (a: t_Slice u8) -> deserialize_4_ a);
+    f_serialize_5_pre = (fun (a: Libcrux_ml_kem.Vector.Portable.t_PortableVector) -> true);
+    f_serialize_5_post
+    =
+    (fun (a: Libcrux_ml_kem.Vector.Portable.t_PortableVector) (out: t_Array u8 (sz 10)) -> true);
+    f_serialize_5_ = (fun (a: Libcrux_ml_kem.Vector.Portable.t_PortableVector) -> serialize_5_ a);
+    f_deserialize_5_pre = (fun (a: t_Slice u8) -> true);
+    f_deserialize_5_post
+    =
+    (fun (a: t_Slice u8) (out: Libcrux_ml_kem.Vector.Portable.t_PortableVector) -> true);
+    f_deserialize_5_ = (fun (a: t_Slice u8) -> deserialize_5_ a);
+    f_serialize_10_pre = (fun (a: Libcrux_ml_kem.Vector.Portable.t_PortableVector) -> true);
+    f_serialize_10_post
+    =
+    (fun (a: Libcrux_ml_kem.Vector.Portable.t_PortableVector) (out: t_Array u8 (sz 20)) -> true);
+    f_serialize_10_ = (fun (a: Libcrux_ml_kem.Vector.Portable.t_PortableVector) -> serialize_10_ a);
+    f_deserialize_10_pre = (fun (a: t_Slice u8) -> true);
+    f_deserialize_10_post
+    =
+    (fun (a: t_Slice u8) (out: Libcrux_ml_kem.Vector.Portable.t_PortableVector) -> true);
+    f_deserialize_10_ = (fun (a: t_Slice u8) -> deserialize_10_ a);
+    f_serialize_11_pre = (fun (a: Libcrux_ml_kem.Vector.Portable.t_PortableVector) -> true);
+    f_serialize_11_post
+    =
+    (fun (a: Libcrux_ml_kem.Vector.Portable.t_PortableVector) (out: t_Array u8 (sz 22)) -> true);
+    f_serialize_11_ = (fun (a: Libcrux_ml_kem.Vector.Portable.t_PortableVector) -> serialize_11_ a);
+    f_deserialize_11_pre = (fun (a: t_Slice u8) -> true);
+    f_deserialize_11_post
+    =
+    (fun (a: t_Slice u8) (out: Libcrux_ml_kem.Vector.Portable.t_PortableVector) -> true);
+    f_deserialize_11_ = (fun (a: t_Slice u8) -> deserialize_11_ a);
+    f_serialize_12_pre = (fun (a: Libcrux_ml_kem.Vector.Portable.t_PortableVector) -> true);
+    f_serialize_12_post
+    =
+    (fun (a: Libcrux_ml_kem.Vector.Portable.t_PortableVector) (out: t_Array u8 (sz 24)) -> true);
+    f_serialize_12_ = (fun (a: Libcrux_ml_kem.Vector.Portable.t_PortableVector) -> serialize_12_ a);
+    f_deserialize_12_pre = (fun (a: t_Slice u8) -> true);
+    f_deserialize_12_post
+    =
+    (fun (a: t_Slice u8) (out: Libcrux_ml_kem.Vector.Portable.t_PortableVector) -> true);
+    f_deserialize_12_ = (fun (a: t_Slice u8) -> deserialize_12_ a);
+    f_rej_sample_pre = (fun (a: t_Slice u8) (out: t_Slice i16) -> true);
+    f_rej_sample_post
+    =
+    (fun (a: t_Slice u8) (out: t_Slice i16) (out2: (t_Slice i16 & usize)) -> true);
+    f_rej_sample
+    =
+    fun (a: t_Slice u8) (out: t_Slice i16) ->
+      let tmp0, out1:(t_Slice i16 & usize) = rej_sample a out in
+      let out:t_Slice i16 = tmp0 in
+      let hax_temp_output:usize = out1 in
+      out, hax_temp_output <: (t_Slice i16 & usize)
+  }
